\documentclass{article}
\begin{document}
Partial Fraction -- Mathematica: {\tt Apart[ 1/((4 n + 1) (4 n - 3))]}
\begin{eqnarray*}
&&
\sum_{n=0}^\infty \frac{1}{(4 n + 1) (4 n - 3)} \\
&&
=
\frac{1}{4}
\left[
\sum_{n=0}^\infty \frac{1}{4 n - 3}
-
\sum_{n=0}^\infty \frac{1}{4 n + 1}
\right] \\
&&\textrm{ index  change in first sum: }\; 4m+1=4n-3 \Rightarrow n= m+1, m=n-1]\\
&&
=
\frac{1}{4}
\left[
\sum_{m=-1}^\infty \frac{1}{4 m + 1}
-
\sum_{n=0}^\infty \frac{1}{4 n + 1}
\right] \\
&&\textrm{ index change in first sum: }\; m=n ]\\
&&
=
\frac{1}{4}
\left[
\sum_{n=-1}^\infty \frac{1}{4 n + 1}
-
\sum_{n=0}^\infty \frac{1}{4 n + 1}
\right] \\
&&
=
\frac{1}{4}
\left[
\frac{1}{4 (-1) + 1}  +
\sum_{n=0}^\infty \frac{1}{4 n + 1}
-
\sum_{n=0}^\infty \frac{1}{4 n + 1}
\right] \\
&&
=
\frac{1}{4}
\left[
\frac{1}{(-3)}  +
0
\right] = - \frac{1}{12}\\
&&
\left\{\textrm{ and, by the way, } =\ldots = \sum_{n=0}^\infty n \right\}\\
\end{eqnarray*}
\end{document}
